refine overrun callback spec; proof skeleton

src/Lib/VstCallback.v
@@ -1,6 +1,7 @@
 Require Import Core.Core.
 Require Import VST.floyd.proofauto.
-Require Import Clight.asn_application.
+Require Import VST.floyd.library.
+Require Import Clight.asn_application Lib.Stdlib.
 
 Definition Vprog : varspecs. mk_varspecs prog. Defined.
 Instance CompSpecs : compspecs. make_compspecs prog. Defined.
@@ -15,35 +16,104 @@ Definition mk_enc_key buf size comp_size : reptype enc_key_s :=
   (buf, (Vint (Int.repr size), Vint (Int.repr comp_size))). 
 
 Definition callback  : funspec :=
-    WITH b : bool, data : list int, data_p : val, size : Z,
+    WITH data : list int, data_p : val, size : Z,
          app_key : val, app_key_p : val, 
          buf_b : block, buf_ofs : ptrofs,
          buf_size : Z, computed_size : Z
     PRE [tptr tvoid, tuint, tptr tvoid]
-      PROP ()
+      PROP (size = Zlength data)
       PARAMS (data_p; Vint (Int.repr size); app_key_p)
       GLOBALS ()
       SEP (data_at Tsh (tarray tuchar (Zlength data)) (map Vint data) data_p;
            data_at Tsh enc_key_s 
                    (mk_enc_key (Vptr buf_b buf_ofs) buf_size computed_size) 
                    app_key_p;
-           data_at_ Tsh tvoid (Vptr buf_b buf_ofs))
+           memory_block Tsh buf_size (Vptr buf_b buf_ofs))
     POST [tint]
       PROP ()
       LOCAL (temp ret_temp Vzero)
       SEP (data_at Tsh (tarray tuchar (Zlength data)) (map Vint data) data_p;
-           data_at Tsh (tarray tuchar (Zlength data)) (map Vint data) 
-                   (Vptr buf_b (Ptrofs.add buf_ofs (Ptrofs.repr computed_size))); 
-           data_at Tsh enc_key_s 
-                  (mk_enc_key (Vptr buf_b buf_ofs) buf_size size) app_key_p).
+           if buf_size <? computed_size + size 
+           then memory_block Tsh buf_size (Vptr buf_b buf_ofs) *
+                data_at Tsh enc_key_s 
+                   (mk_enc_key (Vptr buf_b buf_ofs) 0 computed_size) 
+                   app_key_p
+           else 
+             (data_at Tsh 
+                      (tarray tuchar size) (map Vint data) 
+                      (Vptr buf_b (Ptrofs.add buf_ofs (Ptrofs.repr computed_size))) * 
+              data_at Tsh enc_key_s 
+                      (mk_enc_key (Vptr buf_b buf_ofs)
+                                  buf_size (computed_size + size)) app_key_p)). 
+
+Definition dummy_callback  : funspec :=
+    WITH  data_p : val, size : Z,
+         app_key_p : val
+    PRE [tptr tvoid, tuint, tptr tvoid]
+      PROP ()
+      PARAMS (data_p; Vint (Int.repr size); app_key_p)
+      GLOBALS ()
+      SEP ()
+    POST [tint]
+      PROP ()
+      LOCAL (temp ret_temp Vzero)
+      SEP (). 
 
 Definition callback_overrun_spec : ident * funspec :=
   DECLARE _overrun_encoder_cb callback.
 
-Definition Gprog := ltac:(with_library prog [callback_overrun_spec]).
+Definition Gprog := ltac:(with_library prog [callback_overrun_spec; (_memcpy, memcpy_spec)]).
 
 Theorem bool_der_encode : semax_body Vprog Gprog f_overrun_encoder_cb 
                                      callback_overrun_spec.
+  Proof.
+    start_function.
+    repeat forward; simpl.
+    unfold MORE_COMMANDS.
+    unfold abbreviate.
+    forward_if 
+      (PROP ()
+       LOCAL (temp _t'3 (Vint (Int.repr buf_size)); temp _t'2 (Vint (Int.repr computed_size));
+              temp _key app_key_p; temp _data data_p; temp _size (Vint (Int.repr size));
+              temp _keyp app_key_p)
+       SEP (data_at Tsh (tarray tuchar (Zlength data)) (map Vint data) data_p;
+           if buf_size <? computed_size + size 
+           then memory_block Tsh buf_size (Vptr buf_b buf_ofs) *
+                data_at Tsh enc_key_s 
+                   (mk_enc_key (Vptr buf_b buf_ofs) 0 computed_size) 
+                   app_key_p
+           else 
+             (data_at Tsh 
+                      (tarray tuchar size) (map Vint data) 
+                      (Vptr buf_b (Ptrofs.add buf_ofs (Ptrofs.repr computed_size))) * 
+              data_at Tsh enc_key_s 
+                      (mk_enc_key (Vptr buf_b buf_ofs)
+                                  buf_size (computed_size + size)) app_key_p))).
+    forward.
+    entailer!.
+    admit.
+    repeat forward.
+    (* qsh : share, psh: share, p: val, q: val, n: Z, contents: list int *)
+    forward_call (Tsh, Tsh, Vptr buf_b (Ptrofs.add buf_ofs (Ptrofs.repr computed_size)), data_p,
+                  size, data).
+    entailer!.
+    simpl.
+    admit.
+    entailer!.
+    admit.
+    admit.
+    entailer!.
+    entailer!.
+    admit. 
+    break_if.
+    Intros.
+    repeat forward.
+    entailer!.
+    admit.
+    Intros.
+    repeat forward.
+    entailer!.
+    admit.
 Admitted.
 
 End Encoder_callback. 
