src/Lib/DWT/Vst.v
@@ -27,7 +27,7 @@ Definition der_write_tags_spec : ident * funspec :=
     GLOBALS()
     SEP(data_at_ Tsh type_descriptor_s td_p ; 
         data_at_ Tsh tvoid app_p ;
-        func_ptr' callback cb_p)
+        func_ptr' dummy_callback cb_p)
     POST[tint]
       PROP()
       LOCAL(temp ret_temp 
@@ -37,7 +37,7 @@ Definition der_write_tags_spec : ident * funspec :=
                                   end))))
       SEP(data_at_ Tsh type_descriptor_s td_p ; 
           data_at_ Tsh tvoid app_p ;
-          func_ptr' callback cb_p).
+          func_ptr' dummy_callback cb_p).
 
 Definition Gprog := ltac:(with_library prog [der_write_tags_spec]).
 
